-Adding Beta reduction and began to prove it preserves types

src/Basics.lean
@@ -11,6 +11,8 @@ inductive Typ : Type
   | base : Typ
   | arrow : Typ → Typ → Typ
 
+notation t₁ "->" t₂ => Typ.arrow t₁ t₂ 
+
 -- Print function for convenience --
 def printTyp (t : Typ) : String := by 
   cases t 
@@ -84,6 +86,10 @@ inductive Term : Type
   | abs : Nat → Typ →  Term → Term
   | app : Term → Term → Term
 
+notation "λ (x"n":"t")."te => Term.abs n t te
+notation "$"n":"t => Term.var n t
+notation f"@"t => Term.app f t
+
 def printTerm (t: Term) : String := by
   cases t
   case var n t₁ => exact "x"++(toString n)
@@ -113,15 +119,31 @@ def t₁ : Term := Term.abs 0 base (Term.var 0 base)
 inductive Deduction : Ctx →  Term →  Typ →  Type
   | var (n : Nat) (t : Typ) : Deduction (n,,t ⟶ []) (Term.var n t) t
   | abs {c : Ctx} {t : Term} {ty xt : Typ} {n : Nat} (d : Deduction (n,,xt ⟶ c) t ty) : Deduction c (Term.abs n xt t) (Typ.arrow xt ty)
-  | app {c₁ c₂ : Ctx} { t₁ t₂ : Term} {A B : Typ} (d₁ : Deduction c₁ t₁ (Typ.arrow A B)) (d₂ : Deduction c₂ t₂ A) : Deduction (mergeCtx c₁ c₂) (Term.app t₁ t₂) B
-  | subst (d₁ : Deduction (n₁,,ty₁ ⟶ c₁) t ty) (d₂ : Deduction c₂ t₂ ty₁) : Deduction (mergeCtx c₁ c₂) (substitute n₁ t₂ t) ty
+  | app (c₁ c₂ : Ctx) ( t₁ t₂ : Term) (A B : Typ) (d₁ : Deduction c₁ t₁ (Typ.arrow A B)) (d₂ : Deduction c₂ t₂ A) : Deduction (mergeCtx c₁ c₂) (Term.app t₁ t₂) B
+  | subst (c₁ c₂ : Ctx) (n₁ : Nat) (ty₁ ty : Typ) (t t₂ : Term) (d₁ : Deduction (n₁,,ty₁ ⟶ c₁) t ty) (d₂ : Deduction c₂ t₂ ty₁) : Deduction (mergeCtx c₁ c₂) (t [n₁ // t₂]) ty
 
 notation Γ " ⊢ " t " : " ty => Deduction Γ t ty
 
-theorem ProofId : (0,,base ⟶ []) ⊢ (Term.var 0 base) : base := Deduction.var 0 base
-  
-  
+theorem ProofId : (0,,base ⟶ []) ⊢ ($0:base) : base := Deduction.var 0 base
 
+inductive red : Term → Term → Type
+  | β (n: Nat) (ty : Typ) (t u : Term) : red ((λ (xn:ty).t)@u) (t[n // u])
+
+-- Beta reduction preserves types --
+theorem βTypePreservation {Γ₁ : Ctx} {tt : Typ} {t₁ t₂ : Term} 
+                          (b : red t₁ t₂ ) (d₁ : Γ₁ ⊢ t₁ :tt) : (Γ₁ ⊢ t₂ : tt) := by
+  cases b 
+  case β n ty t₃ u => 
+    let Γ : Ctx := mergeCtx Γ₁ Γ₁ 
+    have : Γ₁ = mergeCtx Γ₁ Γ₁ := sorry
+    rw [this]
+    have d₃ : (n,,ty ⟶ Γ₁) ⊢ t₃ : tt := by
+      sorry
+    have d₄ : Γ₁ ⊢ u : ty := by
+      sorry
+    apply Deduction.subst Γ₁ Γ₁ n ty tt 
+    case d₁ => exact d₃
+    case d₂ => exact d₄ 
 end Term
 end Ctx
 end Typ
